Modifiers/NewOutputs.dfy
@@ -1,0 +1,201 @@
+module Modifiers.NewOutputs {
+
+  import opened Circ
+  import opened Scuf
+  import opened MapFunction
+  import opened Subcircuit
+  import opened ConservedSubcircuit
+  import opened Utils
+  import opened Eval
+
+  function NewOutputsMap(mp: ScufMap, new_outputs: seq<nat>): (r: ScufMap)
+    requires mp.Valid()
+    requires forall i: nat :: i < |new_outputs| ==> new_outputs[i] < |mp.outputs|
+    requires Seq.HasNoDuplicates(new_outputs)
+    ensures r.Valid()
+  {
+    var mapped_outputs := seq(|new_outputs|, (i: nat) requires i < |new_outputs| =>
+      mp.outputs[new_outputs[i]]);
+    reveal Seq.HasNoDuplicates();
+    reveal Seq.ToSet();
+    ScufMap(mp.inputs, mapped_outputs, mp.state)
+  }
+
+  function NewOutputsSF(uf: UpdateFunction, new_outputs: seq<nat>, si: SI): (r: SO)
+    requires uf.Valid()
+    requires forall i: nat :: i < |new_outputs| ==> new_outputs[i] < uf.output_width
+    requires uf.SIVal(si)
+    requires Seq.HasNoDuplicates(new_outputs)
+  {
+    reveal UpdateFunction.Valid();
+    var so := uf.sf(si);
+    var mapped_so_outputs := seq(|new_outputs|, (i: nat) requires i < |new_outputs| => so.outputs[new_outputs[i]]);
+    SO(mapped_so_outputs, so.state)
+  }
+
+  function NewOutputsUpdateFunction(uf: UpdateFunction, new_outputs: seq<nat>): (r: UpdateFunction)
+    requires uf.Valid()
+    requires forall i: nat :: i < |new_outputs| ==> new_outputs[i] < uf.output_width
+    requires Seq.HasNoDuplicates(new_outputs)
+    ensures r.Valid()
+  {
+    var new_sf := (si: SI) requires uf.SIVal(si) => NewOutputsSF(uf, new_outputs, si);
+    reveal UpdateFunction.Valid();
+    UpdateFunction(uf.input_width, |new_outputs|, uf.state_width, new_sf)
+  }
+
+  lemma MFLookupCorrect(c: Circuit, s: Scuf, new_outputs: seq<nat>, np: NP, fi: FI)
+    requires c.Valid()
+    requires s.Valid(c)
+    requires IsIsland(c, s.sc)
+    requires forall i: nat :: i < |new_outputs| ==> new_outputs[i] < s.uf.output_width
+    requires Seq.HasNoDuplicates(new_outputs)
+    requires
+      FIValid(fi, s.mp.inputs, s.mp.state)
+    requires
+      var new_mp := NewOutputsMap(s.mp, new_outputs);
+      np in new_mp.outputs
+    ensures
+      var new_s := NewOutputsScufImpl(c, s, new_outputs);
+      MFLookupOutput(s, fi, np) == MFLookupOutput(new_s, fi, np)
+  {
+    var new_s := NewOutputsScufImpl(c, s, new_outputs);
+    var si := s.mp.fi2si(fi);
+    var new_si := new_s.mp.fi2si(fi);
+    reveal UpdateFunction.Valid();
+    var so := s.uf.sf(si);
+    var new_so := new_s.uf.sf(new_si);
+    assert so.state == new_so.state;
+    assert new_so.outputs == seq(|new_outputs|, (i: nat) requires i < |new_outputs| => so.outputs[new_outputs[i]]);
+    var fo := s.mp.so2fo(so);
+    var new_fo := new_s.mp.so2fo(new_so);
+    var index := Seq.IndexOf(new_s.mp.outputs, np);
+    reveal SeqsToMap();
+    assert FOValid(new_fo, new_s.mp.outputs, new_s.mp.state);
+    reveal Seq.ToSet();
+    assert np in new_fo.outputs;
+    reveal MapMatchesSeqs();
+    assert new_fo.outputs[np] == new_so.outputs[index];
+    assert fo.outputs[np] == new_fo.outputs[np];
+  }
+
+  function NewOutputsScufImpl(c: Circuit, s: Scuf, new_outputs: seq<nat>): (r: Scuf)
+    requires c.Valid()
+    requires s.Valid(c)
+    requires forall i: nat :: i < |new_outputs| ==> new_outputs[i] < s.uf.output_width
+    requires Seq.HasNoDuplicates(new_outputs)
+    ensures r.MapValid()
+  {
+    var new_mp := NewOutputsMap(s.mp, new_outputs);
+    var new_uf := NewOutputsUpdateFunction(s.uf, new_outputs);
+    var new_s := Scuf(s.sc, new_mp, new_uf);
+    assert new_s.MapValid() by {
+      reveal NPsInSc();
+      reveal Seq.ToSet();
+      assert new_s.mp.Valid();
+      assert new_s.mp.InSc(new_s.sc);
+      assert new_s.uf.Valid();
+      assert ScufMapUpdateFunctionConsistent(new_s.mp, new_s.uf);
+    }
+    new_s
+  }
+
+  function NewOutputsScuf(c: Circuit, s: Scuf, new_outputs: seq<nat>): (r: Scuf)
+    requires c.Valid()
+    requires s.Valid(c)
+    requires IsIsland(c, s.sc)
+    requires forall i: nat :: i < |new_outputs| ==> new_outputs[i] < s.uf.output_width
+    requires Seq.HasNoDuplicates(new_outputs)
+    ensures r.Valid(c)
+  {
+    var new_s := NewOutputsScufImpl(c, s, new_outputs);
+    assert new_s.Valid(c) by {
+      assert ScValid(c, new_s.sc);
+      reveal Scuf.SomewhatValid();
+      assert new_s.SomewhatValid(c) by {
+        reveal Scuf.SomewhatValid();
+        reveal ConnOutputs();
+        assert ScValid(c, new_s.sc);
+        assert |ConnOutputs(c, new_s.sc)| == 0 by {
+          IsIslandNoOutputs(c, new_s.sc);
+        }
+        reveal  Seq.ToSet();
+        assert Seq.ToSet(new_s.mp.outputs) <= Seq.ToSet(s.mp.outputs);
+        assert AllONPs(c, new_s.sc) >= Seq.ToSet(new_s.mp.outputs);
+        assert Seq.ToSet(new_s.mp.outputs) >= ConnOutputs(c, new_s.sc);
+        assert (Seq.ToSet(new_s.mp.state) == AllSeq(c, new_s.sc));
+        assert (Seq.ToSet(new_s.mp.inputs) == AllInputs(c, new_s.sc));
+      }
+      reveal Scuf.EvaluatesCorrectly();
+      assert new_s.EvaluatesCorrectly(c) by {
+        reveal Seq.ToSet();
+        forall fi: FI | FIValid(fi, new_s.mp.inputs, new_s.mp.state)
+          ensures
+          && FICircuitValid(c, fi)
+          && (forall np :: np in Seq.ToSet(new_s.mp.outputs) || np in StateINPs(new_s.mp.state) ==>
+            && NPValid(c, np)
+            && (Evaluate(c, np, fi) == EvalOk(MFLookup(new_s, fi, np))))
+        {
+          assert FICircuitValid(c, fi) by {
+            ScufValidFiValidToFICircuitValid(c, new_s, fi);
+            }
+          forall np | np in Seq.ToSet(new_s.mp.outputs) || np in StateINPs(new_s.mp.state)
+            ensures
+              && NPValid(c, np)
+              && (Evaluate(c, np, fi) == EvalOk(MFLookup(new_s, fi, np)))
+          {
+            assert s.EvaluatesCorrectly(c);
+            reveal Seq.ToSet();
+            ScufFOutputsAreValid(c, s);
+            assert Evaluate(c, np, fi) == EvalOk(MFLookup(s, fi, np));
+            if np in StateINPs(new_s.mp.state) {
+              assert Evaluate(c, np, fi) == EvalOk(MFLookup(new_s, fi, np));
+            } else {
+              MFLookupCorrect(c, s, new_outputs, np, fi);
+              assert MFLookupOutput(s, fi, np) == MFLookupOutput(new_s, fi, np) by {
+              }
+              assert Evaluate(c, np, fi) == EvalOk(MFLookup(new_s, fi, np));
+            }
+          }
+        }
+      }
+    }
+    new_s
+  }
+
+  function NewOutputsInserter(c: Circuit, z: ScufInserter, new_outputs: seq<nat>): (r: (Circuit, Scuf))
+    requires c.Valid()
+    requires z.Valid()
+    requires forall i: nat :: i < |new_outputs| ==> new_outputs[i] < z.uf.output_width
+    requires Seq.HasNoDuplicates(new_outputs)
+    ensures
+      var (new_c, new_s) := r;
+      && new_c.Valid()
+      && new_s.Valid(new_c)
+      && SimpleInsertion(c, new_c, new_s)
+  {
+    reveal UpdateFunctionsEquiv();
+    reveal ScufInserter.Valid();
+    var (new_c, s) := z.fn(c);
+    reveal SimpleInsertion();
+    var new_s := NewOutputsScuf(new_c, s, new_outputs);
+    (new_c, new_s)
+  }
+
+  function NewOutputsModifier(z: ScufInserter, new_outputs: seq<nat>): (r: ScufInserter)
+    requires z.Valid()
+    requires forall i: nat :: i < |new_outputs| ==> new_outputs[i] < z.uf.output_width
+    requires Seq.HasNoDuplicates(new_outputs)
+    ensures r.Valid()
+  {
+    reveal ScufInserter.Valid();
+    var new_uf := NewOutputsUpdateFunction(z.uf, new_outputs);
+    var new_z := ScufInserter(
+      new_uf,
+      (c: Circuit) requires c.Valid() => NewOutputsInserter(c, z, new_outputs)
+    );
+    new_z
+  }
+
+
+}
