Modifiers/Series.dfy
@@ -1,0 +1,360 @@
+module ModifiersSeries {
+
+  import opened Circ
+  import opened Scuf
+  import opened MapFunction
+  import opened ConservedSubcircuit
+  import opened SelfConnect
+  import opened Modifiers.Merge
+  import opened Modifiers.Connect
+  import opened Modifiers.NewOutputs
+  import opened Modifiers.SwitchUF
+  import opened Utils
+  import opened Path
+  import opened Subcircuit
+
+  function {:vcs_split_on_every_assert} SeriesInternalConnection(input_width_1: nat, input_width_2: nat, output_width_2: nat): (r: InternalConnection)
+    ensures r.Valid()
+    ensures r.connections.Values == Seq.ToSet(Range(0, input_width_2))
+    ensures r.connections.Keys == Seq.ToSet(Range(input_width_1, input_width_1 + input_width_2))
+  {
+    reveal  Seq.ToSet();
+    var ni_width := input_width_1;
+    var i_width := input_width_1 + input_width_2;
+    var o_width := input_width_2 + output_width_2;
+    var connection_values: seq<nat> := Range(0, input_width_2);
+    var connection_keys: seq<nat> := Range(input_width_1, input_width_1 + input_width_2);
+    assert Seq.HasNoDuplicates(connection_keys) by {
+      reveal Seq.HasNoDuplicates();
+    }
+    var connections: map<nat, nat> := SeqsToMap(connection_keys, connection_values);
+    assert connections.Values == Seq.ToSet(connection_values) by {
+      reveal SeqsToMap();
+      reveal Seq.ToSet();
+      reveal MapMatchesSeqs();
+    }
+    var i2ni := seq(input_width_1, (i: nat) requires i < input_width_1 => i);
+    var nio2i := seq(input_width_1 + input_width_2, (i: nat) requires i < input_width_1 + input_width_2 =>
+      if i < input_width_1 then (false, i) else (true, i - input_width_1));
+    var conn := InternalConnection(ni_width, i_width, o_width, connections, i2ni, nio2i);
+    assert conn.Valid() by {
+      reveal InternalConnection.Valid();
+      reveal Seq.HasNoDuplicates();
+      assert (ni_width <= i_width);
+      assert (i_width <= ni_width + o_width);
+      assert (|i2ni| == ni_width);
+      assert (|nio2i| == i_width);
+      assert Seq.HasNoDuplicates(i2ni);
+      assert Seq.HasNoDuplicates(nio2i);
+      assert (forall index: nat :: index in connections.Values ==> index < o_width);
+      assert (forall index: nat :: index in connections.Keys ==> index < i_width);
+      assert (forall ni_index: nat :: ni_index < ni_width ==> (
+        var i_index: nat := i2ni[ni_index];
+        && (i_index < i_width)
+        && var (from_output, index) := nio2i[i_index];
+        && (!from_output)
+        && (index == ni_index)
+      ));
+      forall i_index: nat | i_index < i_width
+        ensures
+          var (from_output, index) := nio2i[i_index];
+          && ((!from_output) ==> index < ni_width && i2ni[index] == i_index && (i_index !in connections))
+          && ((from_output) ==> index < o_width && (i_index in connections) && (index == connections[i_index]))
+      {
+        var (from_output, index) := nio2i[i_index];
+        if from_output {
+          reveal MapMatchesSeqs();
+          assert i_index >= input_width_1;
+          assert index < o_width;
+          assert index == i_index - input_width_1;
+          InRange(input_width_1, input_width_1 + input_width_2, i_index);
+          assert connection_keys[index] == i_index;
+          assert connection_values[index] == index;
+          assert i_index in connection_keys;
+          assert index == connections[i_index];
+        } else {
+          assert i_index < input_width_1;
+          assert index < ni_width && i2ni[index] == i_index && (i_index !in connections);
+        }
+      }
+    }
+    conn
+  }
+
+  lemma InputsAndOutputsConnected(s: Scuf, input_width_1: nat, input_width_2: nat, output_width_2: nat)
+    requires |s.mp.inputs| == input_width_1 + input_width_2
+    requires |s.mp.outputs| == input_width_2 + output_width_2
+    ensures
+      var conn := SeriesInternalConnection(input_width_1, input_width_2, output_width_2);
+      && (conn.GetConnectedOutputs(s.mp) == Seq.ToSet(s.mp.outputs[..input_width_2]))
+      && (conn.GetConnectedInputs(s.mp) == Seq.ToSet(s.mp.inputs[input_width_1..]))
+  {
+    var connection_values: seq<nat> := Range(0, input_width_2);
+    var connection_keys: seq<nat> := Range(input_width_1, input_width_1 + input_width_2);
+    var conn := SeriesInternalConnection(input_width_1, input_width_2, output_width_2);
+    assert conn.connections.Values == Seq.ToSet(connection_values);
+    reveal Seq.ToSet();
+    assert forall np :: np in conn.GetConnectedOutputs(s.mp) ==> np in Seq.ToSet(s.mp.outputs[..input_width_2]);
+    forall np | np in Seq.ToSet(s.mp.outputs[..input_width_2])
+      ensures np in conn.GetConnectedOutputs(s.mp)
+    {
+      assert np in s.mp.outputs[..input_width_2];
+      var index: nat :| index < input_width_2 && s.mp.outputs[index] == np;
+      InRange(0, input_width_2, index);
+      assert index in connection_values;
+      assert np in conn.GetConnectedOutputs(s.mp);
+    }
+    assert forall np :: np in conn.GetConnectedInputs(s.mp) ==> np in Seq.ToSet(s.mp.inputs[input_width_1..]);
+    forall np | np in Seq.ToSet(s.mp.inputs[input_width_1..])
+      ensures np in conn.GetConnectedInputs(s.mp)
+    {
+      assert np in s.mp.inputs[input_width_1..];
+      var index: nat :| index >= input_width_1 && index < input_width_1 + input_width_2 && s.mp.inputs[index] == np;
+      InRange(input_width_1, input_width_1 + input_width_2, index);
+      assert index in connection_keys;
+      assert np in conn.GetConnectedInputs(s.mp);
+    }
+  }
+
+  function SeriesSF(uf1: UpdateFunction, uf2: UpdateFunction, si: SI): (so: SO)
+    requires uf1.Valid()
+    requires uf2.Valid()
+    requires uf2.input_width == uf1.output_width
+    requires |si.inputs| == uf1.input_width
+    requires |si.state| == uf1.state_width + uf2.state_width
+    ensures |so.outputs| == uf2.output_width
+    ensures |so.state| == uf1.state_width + uf2.state_width
+  {
+    reveal UpdateFunction.Valid();
+    var si1_state := si.state[..uf1.state_width];
+    var si2_state := si.state[uf1.state_width..];
+    var si1 := SI(si.inputs, si1_state);
+    assert |si1.inputs| == uf1.input_width;
+    assert |si1.state| == uf1.state_width;
+    var so1 := uf1.sf(si1);
+    var si2 := SI(so1.outputs, si2_state);
+    assert |si2.inputs| == uf2.input_width;
+    assert |si2.state| == uf2.state_width;
+    var so2 := uf2.sf(si2);
+    var so := SO(so2.outputs, so1.state + so2.state);
+    so
+  }
+
+  function SeriesStep2UpdateFunction(uf1: UpdateFunction, uf2: UpdateFunction): (step2_uf: UpdateFunction)
+    requires uf1.Valid()
+    requires uf2.Valid()
+    requires uf1.output_width == uf2.input_width
+    ensures step2_uf.Valid()
+    ensures step2_uf.input_width == uf1.input_width
+    ensures step2_uf.output_width == uf1.output_width + uf2.output_width
+    ensures step2_uf.state_width == uf1.state_width + uf2.state_width
+    ensures step2_uf.Valid()
+  {
+    var step1_uf := MergeUpdateFunctions(uf1, uf2);
+    reveal MergeUpdateFunctions();
+    var conn := SeriesInternalConnection(uf1.input_width, uf2.input_width, uf2.output_width);
+    assert conn.o_width == uf2.input_width + uf2.output_width;
+    var step2_uf := ConnectUpdateFunction(step1_uf, conn);
+    step2_uf
+  }
+
+  function SeriesStep2ModelSF(uf1: UpdateFunction, uf2: UpdateFunction, si: SI): (so: SO)
+    requires uf1.Valid()
+    requires uf2.Valid()
+    requires uf1.output_width == uf2.input_width
+    requires |si.inputs| == uf1.input_width
+    requires |si.state| == uf1.state_width + uf2.state_width
+    ensures |so.outputs| == uf1.output_width + uf2.output_width
+    ensures |so.state| == uf1.state_width + uf2.state_width
+  {
+    reveal UpdateFunction.Valid();
+    var si1 := SI(si.inputs, si.state[..uf1.state_width]);
+    var so1 := uf1.sf(si1);
+    var si2 := SI(so1.outputs, si.state[uf1.state_width..]);
+    var so2 := uf2.sf(si2);
+    var so := SO(so1.outputs + so2.outputs, so1.state + so2.state);
+    so
+  }
+
+  function SeriesStep2ModelUpdateFunction(uf1: UpdateFunction, uf2: UpdateFunction): (step2m_uf: UpdateFunction)
+    requires uf1.Valid()
+    requires uf2.Valid()
+    requires uf1.output_width == uf2.input_width
+    ensures step2m_uf.Valid()
+  {
+    reveal UpdateFunction.Valid();
+    var new_uf := UpdateFunction(
+      uf1.input_width,
+      uf1.output_width + uf2.output_width,
+      uf1.state_width + uf2.state_width,
+      (si: SI) requires |si.inputs| == uf1.input_width && |si.state| == uf1.state_width + uf2.state_width
+        => SeriesStep2ModelSF(uf1, uf2, si)
+    );
+    new_uf
+  }
+
+  lemma SeriesStep2UpdateFunctionEquiv(uf1: UpdateFunction, uf2: UpdateFunction)
+    requires uf1.Valid()
+    requires uf2.Valid()
+    requires uf2.input_width == uf1.output_width
+    ensures UpdateFunctionsEquiv(SeriesStep2UpdateFunction(uf1, uf2), SeriesStep2ModelUpdateFunction(uf1, uf2))
+  {
+    reveal UpdateFunctionsEquiv();
+    var step2_uf := SeriesStep2UpdateFunction(uf1, uf2);
+    var step2m_uf := SeriesStep2ModelUpdateFunction(uf1, uf2);
+    reveal UpdateFunction.Valid();
+    var conn := SeriesInternalConnection(uf1.input_width, uf2.input_width, uf2.output_width);
+    forall si | step2_uf.SIVal(si)
+      ensures step2_uf.sf(si) == step2m_uf.sf(si)
+    {
+      var si1 := SI(si.inputs, si.state[..uf1.state_width]);
+      var so1 := uf1.sf(si1);
+      var si2 := SI(so1.outputs, si.state[uf1.state_width..]);
+      var so2 := uf2.sf(si2);
+      var uf_merged := MergeUpdateFunctions(uf1, uf2);
+      var si_merged := SI(si.inputs + so1.outputs, si.state);
+      var so_merged := uf_merged.sf(si_merged);
+      assert so_merged == SO(so1.outputs + so2.outputs, so1.state + so2.state) by {
+        reveal MergeUpdateFunctions();
+      }
+      assert so_merged == step2m_uf.sf(si);
+      assert conn.SNI2SOSecondPass(uf_merged, si) == step2_uf.sf(si);
+      // For the first pass we feed all zeros into uf2.
+      var fake_input := seq(uf2.input_width, (index: nat) requires index < uf2.input_width => false);
+      var si2_fake := SI(fake_input, si2.state);
+      var so2_fake := uf2.sf(si2_fake);
+      var so_first_pass := SO(so1.outputs + so2_fake.outputs, so1.state + so2_fake.state);
+      var si_merged_fake := SI(si.inputs + fake_input, si.state);
+      var so_merged_first_pass := uf_merged.sf(si_merged_fake);
+      assert so_first_pass == so_merged_first_pass by {
+        reveal MergeUpdateFunctions();
+      }
+      assert conn.SNI2SOFirstPass(uf_merged, si) == so_first_pass by {
+        var fake_outputs := seq(uf1.output_width + uf2.output_width, (index: nat) requires index < uf1.output_width + uf2.output_width => false);
+        assert conn.SNI2SIFromOutputs(si, fake_outputs) == SI(si.inputs + fake_input, si.state);
+        reveal MergeUpdateFunctions();
+      }
+      assert conn.SNI2SOSecondPass(uf_merged, si) == so_merged by {
+        var si_second_pass := conn.SNI2SIFromOutputs(si, so_first_pass.outputs);
+        assert si_second_pass == si_merged;
+      }
+      assert so_merged == step2_uf.sf(si);
+      assert step2_uf.sf(si) == step2m_uf.sf(si);
+    }
+  }
+
+  function SeriesStep3UpdateFunction(uf1: UpdateFunction, uf2: UpdateFunction): (step3_uf: UpdateFunction)
+    requires uf1.Valid()
+    requires uf2.Valid()
+    requires uf1.output_width == uf2.input_width
+    ensures step3_uf.Valid()
+    ensures step3_uf.output_width == uf2.output_width
+    ensures step3_uf.input_width == uf1.input_width
+    ensures step3_uf.state_width == uf1.state_width + uf2.state_width
+  {
+    var step2_uf := SeriesStep2UpdateFunction(uf1, uf2);
+    var new_outputs := SeriesNewOutputs(uf1.output_width, uf2.output_width);
+    var step3_uf := NewOutputsUpdateFunction(step2_uf, new_outputs);
+    step3_uf
+  }
+
+  function SeriesUpdateFunction(uf1: UpdateFunction, uf2: UpdateFunction): (new_uf: UpdateFunction)
+    requires uf1.Valid()
+    requires uf2.Valid()
+    requires uf2.input_width == uf1.output_width
+    ensures new_uf.Valid()
+  {
+    reveal UpdateFunction.Valid();
+    UpdateFunction(
+      uf1.input_width,
+      uf2.output_width,
+      uf1.state_width + uf2.state_width,
+      (si: SI) requires |si.inputs| == uf1.input_width && |si.state| == uf1.state_width + uf2.state_width
+        => SeriesSF(uf1, uf2, si)
+    )
+  }
+
+  lemma SeriesUpdateFunctionEquiv(uf1: UpdateFunction, uf2: UpdateFunction)
+    requires uf1.Valid()
+    requires uf2.Valid()
+    requires uf2.input_width == uf1.output_width
+    ensures UpdateFunctionsEquiv(SeriesUpdateFunction(uf1, uf2), SeriesStep3UpdateFunction(uf1, uf2))
+  {
+    SeriesStep2UpdateFunctionEquiv(uf1, uf2);
+    reveal UpdateFunctionsEquiv();
+  }
+
+  function SeriesNewOutputs(output_width_1: nat, output_width_2: nat): (new_outputs: seq<nat>)
+    ensures forall i: nat :: i < |new_outputs| ==> new_outputs[i] < output_width_1 + output_width_2
+    ensures Seq.HasNoDuplicates(new_outputs)
+  {
+    reveal Seq.HasNoDuplicates();
+    seq(output_width_2, (i: nat) requires i < output_width_2 => output_width_1 + i)
+  }
+
+  function SeriesModifier(z1: ScufInserter, z2: ScufInserter): (new_z: ScufInserter)
+    requires z1.Valid()
+    requires z2.Valid()
+    requires z1.uf.output_width == z2.uf.input_width
+    ensures new_z.Valid()
+  {
+
+    reveal UpdateFunctionsEquiv();
+    reveal ScufInserter.Valid();
+    reveal SimpleInsertion();
+    var z_merged := MergeModifier(z1, z2);
+    var conn := SeriesInternalConnection(z1.uf.input_width, z2.uf.input_width, z2.uf.output_width);
+    assert InserterConnectionConsistent(z_merged, conn) by {
+      assert UFConnectionConsistent(z_merged.uf, conn) by {
+        reveal MergeUpdateFunctions();
+      }
+      forall c: Circuit | c.Valid()
+        ensures
+          var (new_c, s) := z_merged.fn(c);
+          ScufConnectionConsistent(new_c, s, conn)
+      {
+        z_merged.ValidForCircuit(c);
+        var (new_c, s) := z_merged.fn(c);
+        //var conn_outputs := conn.GetConnectedOutputs(s.mp);
+        //var conn_inputs := conn.GetConnectedInputs(s.mp);
+        assert new_c.Valid() && s.Valid(new_c) by {
+          reveal SimpleInsertion();
+        }
+        assert ScufConnectionConsistent(new_c, s, conn) by {
+          assert (conn.i_width == s.uf.input_width);
+          assert (conn.o_width == s.uf.output_width);
+          MergeModifierPathConstraints(z1, z2, c);
+          InputsAndOutputsConnected(s, z1.uf.input_width, z2.uf.input_width, z2.uf.output_width);
+          reveal Seq.ToSet();
+          assert conn.GetConnectedOutputs(s.mp) == Seq.ToSet(s.mp.outputs[..z1.uf.output_width]);
+          assert !PathExistsBetweenNPSets(new_c, conn.GetConnectedOutputs(s.mp), conn.GetConnectedInputs(s.mp));
+          assert forall x :: (x in s.mp.inputs) ==> (x !in new_c.PortSource) by {
+            FInputsInSc(new_c, s);
+            reveal NPsInSc();
+            IsIslandNoInputs(new_c, s.sc);
+            assert forall x: NP :: (x in s.mp.inputs) ==> (x.n in s.sc);
+            reveal ConnInputs();
+            reveal UnconnInputs();
+            reveal Scuf.SomewhatValid();
+            reveal Seq.ToSet();
+            assert forall x: NP :: (x in s.mp.inputs) ==> x in AllInputs(new_c, s.sc);
+          }
+          assert (forall i_index :: i_index in conn.connections ==> s.mp.inputs[i_index] !in new_c.PortSource);
+          reveal ScufConnectionConsistent();
+        }
+      }
+      reveal InserterConnectionConsistent();
+    }
+    var z_connected := ConnectModifier(z_merged, conn);
+    var new_outputs := SeriesNewOutputs(z1.uf.output_width, z2.uf.output_width);
+    assert z_connected.uf.output_width == z1.uf.output_width + z2.uf.output_width by {
+      reveal MergeUpdateFunctions();
+    }
+    var z_new_outputs := NewOutputsModifier(z_connected, new_outputs);
+    var new_uf := SeriesUpdateFunction(z1.uf, z2.uf);
+    SeriesUpdateFunctionEquiv(z1.uf, z2.uf);
+    var z_final := SwitchUFModifier(z_new_outputs, new_uf);
+    z_final
+  }
+
+}
