Modifiers/SwitchUF.dfy
@@ -1,0 +1,55 @@
+module Modifiers.SwitchUF {
+
+  import opened Circ
+  import opened Scuf
+  import opened MapFunction
+  import opened ConservedSubcircuit
+
+  function SwitchUFInserter(c: Circuit, z: ScufInserter, uf: UpdateFunction): (r: (Circuit, Scuf))
+    requires c.Valid()
+    requires z.Valid()
+    requires uf.Valid()
+    requires
+      reveal ScufInserter.Valid();
+      UpdateFunctionsEquiv(uf, z.uf)
+    ensures
+      var (new_c, new_s) := r;
+      && new_c.Valid()
+      && new_s.Valid(new_c)
+      && SimpleInsertion(c, new_c, new_s)
+  {
+    reveal UpdateFunctionsEquiv();
+    reveal ScufInserter.Valid();
+    reveal SimpleInsertion();
+    var (new_c, s) := z.fn(c);
+    var new_s := Scuf(s.sc, s.mp, uf);
+    assert new_s.Valid(new_c) by {
+      reveal Scuf.SomewhatValid();
+      assert new_s.SomewhatValid(new_c);
+      assert new_s.SomewhatValidRelaxInputs(new_c) by {
+        new_s.SomewhatValidToRelaxInputs(new_c);
+      }
+      assert new_s.EvaluatesCorrectly(new_c) by {
+        reveal Scuf.EvaluatesCorrectly();
+      }
+    }
+    (new_c, new_s)
+  }
+
+  function SwitchUFModifier(z: ScufInserter, uf: UpdateFunction): (r: ScufInserter)
+    requires z.Valid()
+    requires uf.Valid()
+    requires
+      reveal ScufInserter.Valid();
+      UpdateFunctionsEquiv(uf, z.uf)
+    ensures r.Valid()
+  {
+    reveal ScufInserter.Valid();
+    var new_z := ScufInserter(
+      uf,
+      (c: Circuit) requires c.Valid() => SwitchUFInserter(c, z, uf)
+    );
+    new_z
+  }
+
+}
